

# MATH210: Discrete Mathematics

Mateo Armijo

November 2025

## 1 Relations

Definition: Let  $A$  and  $B$  be sets

A relation from  $A$  to  $B$  is a subset  $R \subseteq A \times B$

Notation: if  $(a, b) \in R$  we sometimes write  $aRb$

Definition:  $R$  is a relations on  $A$  if  $R \subseteq A \times A$

Example:  $A = \{1, 2, 3\}, B = \{a, b, c, d\}$

$R_1 = \{(1, a), (1, b), (2, b), (3, c)\}$

$R_2 = \{(1, a), (1, b), (1, c)\}$

$R_3 = \{(1, b), (2, d)\}$

are all relations From  $A$  to  $B$

Definition: Let  $R$  be a relations on  $A$

(i)  $R$  is reflexive if  $\forall a \in A, (a, a) \in R$

(ii)  $R$  is transitive if  $(a, b) \in R, (b, c) \in R \implies (a, c) \in R$

(iii)  $R$  is symmetric if  $(a, b) \in R \implies (b, a) \in R$

(iv)  $R$  is antisymmetric if  $(a, b) \in R \wedge (b, a) \in R \implies a = b$

Example: Consider  $D \subseteq \mathbb{N} \times \mathbb{N}$  where

$$(a, b) \in D \iff \overset{Defn}{a|b} \iff b = ak, k \in \mathbb{Z}$$

we can see  $(4, 12) \in D, (5, 8) \notin D, (3, 15) \in D \dots$

Claim:  $D$  is reflexive

Proof: Yes are we take  $k = 1$  then  $a = a \implies a|a \implies (a, a) \in D$

Claim:  $D$  is transitive

Proof: Suppose that  $(a, b) \in D, (b, c) \in D$

$$\implies b = ak, c = bl, k, l \in \mathbb{Z} \implies c = ak l \implies a|c \implies (a, c) \in D$$

Claim:  $D$  is not symmetric

Proof: Indeed,  $(1, 2) \in D, (2, 1) \notin D$

Claim:  $D$  is anti symmetric

Proof: Let  $a, b \in \mathbb{N}$ ,

Suppose that  $(a, b) \in D, (b, a) \in D$

$$\implies a = bk, b = al \implies b = bkl \implies a(1 - kl) = 0$$

$$\implies k = l = 1$$

So  $a = b$

Example: Consider  $A = \mathbb{N}$

$$(m, n) \in l \iff (\exists k \in \mathbb{N}_0) : m = n + k$$

Claim:  $l$  is reflexive,

Proof: Let  $a \in \mathbb{N}$

take  $k = 0 \implies a = a + 0$

Claim:  $l$  is transitive,

Proof: Given  $(a, b) \in l, (b, c) \in l$

$$\implies a + k = b, b + i = c$$

Set  $j = i + k$

$$\implies a + i = a + k + i = b + i + c$$

Claim:  $l$  is not symmetric

Proof:  $(4, 3) \notin l, (3, 4) \in l$

Claim:  $l$  is anti symmetric

Proof: Given  $(a, b) \in l, (b, a) \in l$

$$\implies a + k = b, b + l = a \implies b + l + k = b \implies l = -k \implies l = k = 0 \implies a = b$$

## 1.1 Orderings

Definition: Let  $X \neq \emptyset$  be a set and  $R$  a relation on  $X$

if  $R$  is reflexive, transitive, and antisymmetric

then  $R$  is called an ordering or a partial ordering on  $X$

We call the pair  $(X, R)$  a partially ordered set or an ordered set.

Example:  $(\mathbb{N}, D), (\mathbb{N}, l)$  are both ordered sets.

Notation: If  $(X, R)$  is an ordered sets, we write  $(X, \leq_R)$

Example: Let  $S \neq \emptyset$

We can define two orderings on  $\mathcal{P}(S)$

$$(A, B) \in I \iff A \subseteq B \text{ We call this the Inclusion ordering}$$

$$(A, B) \in R \iff A \supseteq B \text{ We call this the reverse inclusion ordering}$$

Definition: Let  $(X, R)$  be an ordered set,  $R$  is total or Linear if  $\forall a, b \in X$  either

$$(a, b) \in R \vee (b, a) \in R$$

Example:

(i)  $(\mathbb{N}, L)$  is total

(ii)  $(\mathbb{N}, D)$  is not total

(iii)  $(\mathcal{P}(S), \subseteq)$  is not total unless  $S$  has one element

(iv)  $(\mathcal{P}(S), \supseteq)$  is not total unless  $S$  has one element

Remark: Let  $(X, \leq)$  be an ordered set and  $Y \subseteq X$ , then  $(Y, \leq)$  is also an ordered

set.

Definition: Let  $(X, \leq)$  be an ordered set, suppose  $A \subseteq X$

(i)  $A$  is bounded above  $\iff (\exists u \in X) : (\forall a \in A)(a \leq u)$

(ii)  $A$  is bounded below  $\iff (\exists u \in X) : (\forall a \in A)(a \geq u)$

(iii) If  $u$  is an upper bound of  $A$  and  $u \in A$  then  $u = \text{greatest}\{A\}$  or the greatest element of  $A$

(iv) If  $l$  is a lower bound of  $A$  and  $l \in A$  then  $l = \text{least}\{A\}$  or the least element of  $A$

Example:  $(\mathbb{N}, D), A = \{5, 12, 16\}$

We see that  $5 \cdot 12 \cdot 16$  is an upper bound

Example:  $(\mathcal{P}(S), \subseteq)$  suppose  $W = \{A, B, C\} \subseteq \mathcal{P}(S)$

We see that  $A$  lower bound of  $W$  is  $\emptyset$  and also  $A \cap B \cap C$

similarly,  $A \cup B \cup C$  is also an upper bound

Definition: A directed graph is a pair  $(V, E)$  of Sets with  $E \subseteq V \times V$

$V$  is the set of vertices and  $E$  is the set of Edges

if  $e \in E$  is an edge from  $a$  to  $b$

$e = (a, b)$

So given a relation we can consider the directed graph and given a directed graph we can find a relations

e.g.  $R \subseteq A \times A$  we take  $V = A, E = R$

Example: (Ordering of functions)

Consider  $\mathcal{F}(\mathbb{R}) = \{f \mid f : \mathbb{R} \rightarrow \mathbb{R}\}$

$$f \leq g \iff \forall x \in \mathbb{R}, f(x) \leq g(x)$$

We see that it is reflexive since  $\forall x, f(x) \leq f(x)$

this is transitive because if  $\forall x \in \mathbb{R}$  we have  $f(x) \leq g(x) \leq h(x) \implies f \leq h$

this is anti symmetric since if  $f(x) \leq g(x), g(x) \leq f(x)$  we must have  $f(x) = g(x)$

This is not total since  $\cos(x), \sin(x)$

Definition: Let  $(X, \leq)$  be an ordered set,  $\leq$  is directed if  $\forall a, b \in X, \exists c \in X : c \geq a, c \geq b$

Example: We see that  $(\mathbb{N}, \leq_D)$  is directed since for any two  $m, n \in \mathbb{N}$  we consider  $p = mn$  then  $p \mid m, p \mid n$

Example: Same with the power set and inclusion we can consider  $A \cup B$

Example: We consider  $(\mathcal{F}(\mathbb{R}), \leq)$ . This is directed since given  $f, g$  we can consider  $h : \mathbb{R} \rightarrow \mathbb{R}, h(x) = \max\{f(x), g(x)\}$

Example: Let  $(X, \leq)$  be an ordered set that is directed.

If  $A \subseteq X$  is finite then  $A$  is bounded above

Proof: We will perform induction on the number of elements in  $A$ .

$A_n = \{a_1, a_2, \dots, a_n\}$

Base Case  $n = 1$ , we see that the upper bound of  $A_1$  is  $a_1$

For  $n = 2$  we can use the directedness of  $X$  to find  $u \in X : u > a_1, u > a_2$

Suppose for some  $|A| = m$  we can find an upper bound

Indeed, for  $|A_{m+1}| = m + 1$  we write  $A_{m+1} = A_m \cup \{a_{m+1}\}$  Using our induc-

tion hypothesis we can find an upper bound of  $A_m$  then we use directedness for find an upper bound of the set containing the upper bound of  $A_m$  and  $a_{m+1}$

Definition: Let  $(X, \leq)$  be an ordered set,  
if  $(\forall \emptyset \neq A \subseteq X)(\exists l \in A) : (l = \text{least}(A))$   
then we call  $X$  a well ordered set.

e.g.  $\mathbb{N}$

Definition: Let  $(X, \leq)$  be an ordered set, and  $A \subseteq X$

(i)  $M \in A$  is maximal if  $\forall a \in A$  we have  $a \geq M \implies M = a$

(ii)  $M \in A$  is minimal if  $\forall a \in A$  we have  $a \leq M \implies M = a$

Example:  $(\mathbb{N}, \leq_D)$

$$m \leq_D n \iff m|n \iff \exists k \in \mathbb{Z} : n = km$$

$A = \{1, 2, 3, 4, 7, 10\}$

Bounded above? Yes take  $2 \cdot 3 \cdot 7 \cdot 5$

If does not have a greatest element but has maximal elements,

Yes 3, 4, 7, 10

Does it have a least element?

Yes 1

Does it have a minimal element?

Yes 1

Definition: Let  $(X, \leq)$  be an ordered set.

Suppose  $A \subseteq X$

(i) If  $u$  is an upper bound of  $A$  and  $u \leq v$  where  $v$  is any upperbound of  $A$  then  $u := \sup(A)$  or the least upper bound of  $A$

(ii) If  $u$  is a lower bound of  $A$  and  $u \geq v$  where  $v$  is any lowerbound of  $A$  then  $u := \inf(A)$  or the greatest lower bound of  $A$

Example: Take  $(\mathbb{R}, \leq)$   $A = [0, 1)$

We claim that  $A$  does not have a greatest element.

Proof: Suppose for contradiction  $\exists t \in A : t \geq a \forall a \in A$

Since  $t \in A \implies 0 \leq t < 1$

take  $\delta = \frac{1+t}{2}$  then  $t < \delta < 1$  hence  $\delta \in A$

Claim:  $\sup(A) = 1$

Let  $x \in A$  then  $x < 1$

so 1 is an upper bound

Let  $v$  be another upper bound for  $A$ , if  $v > 1$  we are done

if  $v < 1$  consider  $\delta = \frac{1+v}{2}$  then  $v < \delta < 1$  so  $\delta \in A, \delta > v$  so 1 must be the least upper bound.

## 1.2 Equivalence Relations

Definition: Given a relations  $R$  on  $X$

If  $R$  is reflexive, transitive, and symmetric then we call  $R$  an equivalence relation on  $X$

Notation:  $(x, y) \in R \iff x \sim_R y$

Example: Consider the relation on  $\mathbb{Q}$ ,

$$(\mathbb{Q}, \sim_R).R = \{(r, q) \mid r, q \in \mathbb{Q}, r - q \in \mathbb{Z}\}$$

This is non empty since we see that  $(\frac{3}{2}, \frac{1}{2}) \in R$

Now we will now show that  $R$  is an equivalence relation on  $\mathbb{Q}$

Proof:

Claim 1:  $R$  is reflexive,

Proof: given  $r \in \mathbb{Q}$ ,  $r - r = 0 \in \mathbb{Z}$

Claim 2:  $R$  is transitive,

Proof: Given  $(p, q) \in R$ ,  $(q, r) \in R$

We know that  $p - q \in \mathbb{Z}$  and  $q - r \in \mathbb{Z}$  so adding these we get that  $p - q + q - r = p - r \in \mathbb{Z}$

Claim 3:  $R$  is symmetric

Proof: Given  $(p, q) \in R$

we see that  $p - q \in \mathbb{Z}$  so multiplying by  $(-1)$  we find that  $q - p \in \mathbb{Z}$

Example: This will be our running example to motivate our study of probability

$$\Omega := \{(n_k)_{k=1}^\infty \mid n_k \in \{0, 1\}\}$$

$$(a_k)_k \sim (b_k)_k \iff (\exists N \in \mathbb{N})(\forall k \geq N)(a_k = b_k)$$

We call  $\Omega$  the coin flip space and we say that this equivalence relation is the tail equivalency,

We claim that  $\sim$  is an equivalence relation,

Proof:

Claim 1: Reflexive

Pf: Clearly we just take  $N = 1$  then  $a_k = a_k \forall k \geq 1$

Claim 2: Transitive

Pf: Given  $(a_k)_k \sim (b_k)_k$ ,  $(b_k)_k \sim (c_k)_k$

$$\implies (\exists N_1 \in \mathbb{N}) : (\forall k \geq N_1)(a_k = b_k)$$

$$\implies (\exists N_2 \in \mathbb{N}) : (\forall k \geq N_2)(b_k = c_k)$$

Take  $N = \max\{N_1, N_2\}$

Then

$$\forall k \geq N, a_k = b_k = c_k$$

Claim 3: Symmetric

pf: Just take the same  $N$ ,

### 1.3 Modular Arithmetic

Fix an  $n \geq 1$ , We define an equivalence relation  $\sim_n$  on  $\mathbb{Z}$

$$a \sim_n b \iff n \mid a - b$$

We claim this is an equivalence relation. Proof:

Reflexive?  $a \sim_n a \iff a - a = nk \iff n|0$

Transitive? Suppose that  $a \sim_n b, b \sim_n c$   
then

$$\begin{aligned} a - b &= nk, b - c = nl \\ \iff a - c &= n(k + l) \\ \iff n|a - c &\implies a \sim_n c \end{aligned}$$

Symmetric?

$$\begin{aligned} a \sim_n b &\iff n|a - b \iff a - b = nk, k \in \mathbb{Z} \\ \implies -(a - b) &= n(-k) \implies b - a = n(-k) \implies b \sim_n a \end{aligned}$$

Example: (From  $\mathbb{Z}$  to  $\mathbb{Q}$ ),

Consider  $X = \mathbb{Z} \times \mathbb{N}$  we define  $R \subseteq X \times X$

$$(a, b) \sim (cd) \iff ad = bc$$

We claim that this an equivalence relation

Proof: Reflexive?

$$(a, b) \sim (a, b) \iff ab = ba \iff ab = ab \text{ (Commutativity)}$$

Transitive?

Suppose,  $(a, b) \sim (c, d), (c, d) \sim (e, f)$

We have  $ad = bc, cf = de$

$$afd = bcf = bde \implies d(af - be) = 0 \iff d = 0 \vee (af = be)$$

Since  $b \in \mathbb{N}, b \neq 0$

Hence  $af = be \implies (a, b) \sim (e, f)$  Symmetric?

$$(a, b) \sim (c, d) \iff ad = bc \iff cd = da \iff (c, d) \sim (a, b) \text{ Definition: Let}$$

$R$  be an equivalence relation on a Set  $X$ ,

Let  $x \in X$ .

the set  $[x]_R$  is the called the equivalence class of  $x$

$$[x]_R := \{y \in X \mid y \sim_R x\}$$

Facts:

(i)  $x \in [x]_R$  (Reflexivity)

(ii)  $x \in [y]_R \iff y \in [x]_R$  (Symmetry)

(iii)  $[x]_R = [y]_R \iff x \sim_R y$  (Follows from (ii) and transitivity)

Proof: (iii)

$\implies$ :

$$[x]_R = [y]_R \implies x \in [x]_R = [y]_R \implies x \sim_R y$$

$\Leftarrow$ :

$$z \in [x]_R \iff z \sim x \text{ by transitivity } z \sim y \iff z \in [y]_R$$

We call  $x$  the representative of the class  $[x]_R$ ,

Example: fix  $n = 3$ , we had an equivalence relation on  $\mathbb{Z}$   $a \sim_3 b \iff 3|a - b$   
What does the class of 2 look like?  $[2]_3 = \{m \in \mathbb{Z} \mid m \sim_3 2\}$

$$m \in [2]_3 \iff m \sim_3 2 \iff 3|m - 2 \iff m = 3k + 2$$

Hence  $[2]_3 = \{m \in \mathbb{Z} \mid m = 3k + 2, k \in \mathbb{Z}\} = \{3k + 2 \mid k \in \mathbb{Z}\} = 2 + 3\mathbb{Z}$

What does  $[1]_3$  look like?

$1 + 3\mathbb{Z}$

What does  $[0]_3$  look like?

$3\mathbb{Z}$

Notice we showed in a homework that  $3\mathbb{Z} \cap 3\mathbb{Z} + 1 \cap 3\mathbb{Z} + 2 \neq \emptyset$   
and  $\mathbb{Z} = 3\mathbb{Z} \sqcup 3\mathbb{Z} + 1 \sqcup 3\mathbb{Z} + 2$

Proof:  $([1]_3 \cap [2]_3 = \emptyset)$

Suppose for contradiction  $\exists m \in [1]_3 \cap [2]_3$

$\implies m \sim 1 \wedge m \sim 2 \implies 1 \sim m \sim 2$  (Symmetry)

$\implies 1 \sim 2 \#$  we can find similarly, they are all pairwise disjoint.

Claim:  $\mathbb{Z} \subseteq [0]_3 \sqcup [1]_3 \sqcup [2]_3$

Proof: if  $m = 0, 1, 2$  done so suppose that  $m > 2$

Consider the set  $R = \{m - 3k \mid k \in \mathbb{Z}\} \cap \mathbb{N}_0$

By the well ordering principle,  $\exists l \in R : l = \text{least}(R)$

So  $0 \leq l = m - 3k \implies 3k = m - l \implies 3|m - l \implies m \sim l$

We claim that  $l \in \{0, 1, 2\}$

Pf: Suppose that  $l \geq 3 \implies l = 3 + a, a > 0$

$\implies m - 3k = 3 + a \implies m - 3(k + 1) = a \iff m - 3j = a \implies a \in R$

But we had that  $a < l$  so  $a = \text{least}(R) \#$

Hence we must have that  $m \in [0]_3 \sqcup [1]_3 \sqcup [2]_3$

Proposition: Fix  $n \in \mathbb{N}$

Let  $\sim_n$  be an equivalence relation on  $\mathbb{Z}$

$a \sim_n b \iff n|a - b$

Then,

$$\mathbb{Z} = \bigsqcup_{k=0}^{n-1} [k]_n$$

Proof: fix  $n \in \mathbb{N}$

Claim 1:  $l \neq k \in \{0, 1, \dots, n-1\} \implies [l]_n \cap [k]_n = \emptyset$

Pf:

Suppose for contraction  $m \in [k]_n \cap [l]_n$

$\implies m \sim_n l, m \sim_n k$

$\iff l \sim_n m \sim_n k$  (Symmetry)

$\implies l \sim_n k$

$\implies n|l - k \implies l - k = nj$

So  $|l - k| < n \implies n > |l - k| = nj \geq n$

Claim 2: Given  $m \in \mathbb{Z}, \exists r \in \{0, 1, \dots, n-1\}$  with  $m \in [r]_n$

Proof: If  $m \in \{0, 1, \dots, n-1\}$  done so suppose that  $m \geq n$

Consider  $R_m = \{m - nk \mid k \in \mathbb{Z}\} \cap \mathbb{N}_0$

By well ordering,  $\exists r \in R_m : r = \text{least}(R_m)$

Then  $r \geq 0, r = m - nl, l \in \mathbb{Z}$

Suppose that  $r \geq n \implies r = n + a, a > 0$

Then  $n + a = m - nl \implies a = m - n(1 + l) \implies a \sim m \implies a \in R_m, a \leq r$   
so  $r$  is not the least element.

Proposition: Let  $\sim_R$  be an equivalence relation on  $X$

for any  $[a], [b]$  either  $[a] = [b]$  or  $[a] \cap [b] = \emptyset$

We can also write  $X = \bigsqcup_{i \in I} [x_i]$

Claim:  $(\exists x \in [a] \cap [b]) \implies [a] = [b]$

Proof: Suppose for contradiction,  $(\exists y \in [a], y \notin [b])$

then  $x \sim y \implies y \sim x \sim b \implies y \sim b \implies y \in [b]$

Definition: Let  $A$  be a set, a partition of  $A$  is a family of pairwise disjoint subsets

$\{A_i\}_{i \in I}$  such that  $A = \bigsqcup_{i \in I} A_i$

Example:  $\mathbb{N} = \mathbb{E} \cup \mathbb{O} = [0]_2 \sqcup [1]_2$

Example:  $\mathbb{N} = \bigsqcup_{n \in \mathbb{N}} [n]$

Challenge: Write  $\mathbb{N}$  as the disjoint union of infinite sets.

$\mathbb{N} = \bigsqcup_{n=1}^{\infty} N_k, N_k$  infinite

Proposition: Given a partition  $\bigsqcup_{i \in I} X_i = X$  we can define an equivalence relation on  $X$

$x, y \in X, x \sim y \iff (\exists i \in I) : (x, y \in X_i)$

Definition: Let  $R$  be an equivalence relation on  $X$

(i)  $x \in X, [x]_R = \{y \in X \mid y \sim_R x\}$

(ii)  $X/R = \{[x]_R \mid x \in X\}$

Example:  $\mathbb{Z}/\sim_n = \{[m] \mid m \in \mathbb{Z}\}$

this has  $n$  elements and each element is a class. Point being we wish to do operation on this set.

We want to make an algebra recall, we have  $(\mathbb{N}, \times, +)$  and with  $(\mathbb{Z}, \times, +, -)$

We claim that on  $(\mathbb{Z}/\sim_n)$  has  $[a]_n + [b]_n = [a + b]_n$  is a well defined.

Proof: Suppose we have  $[a']_n = [a]_n$  and  $[b']_n = [b]_n$

$[a']_n = [a]_n \iff a \sim a' \iff n \mid a - a' \iff kn = a - a'$

similarly we have  $ln = b - b' \implies b \mid a + b - a' - b' \iff a + b \sim a' + b' \iff [a + b] = [a' + b']$

### 1.3.1 Forming the Rationals

Consider the Set  $X = \mathbb{Z} \times \mathbb{Z}^*, \mathbb{Z}^* = \mathbb{Z} \setminus \{0\}$

Let  $Q$  be an equivalence relation on  $X$ .

$$(a, b) \sim (c, d) \iff ad = bc$$

We consider  $X/Q := \{[(a, b)] \mid a, b \in \mathbb{Z}, b \neq 0\}$

Claim 1:  $[(a, b)] = \{(an, bn) \mid n \in \mathbb{Z}\}$

e.g.  $[(4, 6)] = \{(2n, 3n) \mid n \in \mathbb{Z}\}$

Proof: Certainly,  $(2n, 3n) \sim (4, 6)$ ,

Now Suppose that  $(x_1, x_2) \in [(4, 6)] \implies (x_1, x_2) \sim (4, 6)$

$\implies 6a - 4b \implies 3a = 2b \implies 3a$  is even



So we write  $a = 2n$ , now we have  $3a = 2n = 2b \implies n = b$

So  $(a, b) \sim (2n, 3n)$

Given  $a, b \in \mathbb{Z}, b \neq 0$  we write  $a = ka', b = kb'$  where  $a'$  and  $b'$  have no common factor.

Claim:  $[(a, b)] = \{(na', nb') \mid n \in \mathbb{Z}, n \neq 0\}$

Now we can define operations on  $\mathbb{Q} := X/Q$

We will verify that  $(\mathbb{Q}, +)$  is well defined.

Proof: Suppose  $[(a, b)] = [(a', b')], [(c, d)] = [(c', d')]$

$$[(a, b)] = [(a', b')] \iff (a, b) \sim (a', b') \implies ab' = a'b$$

Similarly,

$$cd' = c'd$$

So we consider

$$\begin{aligned} bd(a'd') + bd(c'b') &= b'd'(ad) + b'd'(cb) \\ \iff a'bdd' + c'b'bd &= a'd'bd + bdb'c' \\ \iff a'bdd' + b'c'db &= a'd'bd + bdb'c' \\ \iff b'd'(ad + bc) &= bd(a'd' + b'c') \end{aligned}$$

Notice  $(\mathbb{Q}, +), + : \mathbb{Q} \rightarrow \mathbb{Q}$

we have:

- (i)  $a + (b + c) = (a + b) + c$  (Associativity)
- (ii)  $a + 0 = a = 0 + a$  (Additive Identity)
- (iii)  $(\forall q \in \mathbb{Q})(\exists! q^{-1} \in \mathbb{Q}) : q + q^{-1} = 0$  (Additive inverses)
- (iv)  $a + b = b + a$  (Commutativity) This are the requirements for an abelian group.

Now we consider  $\cdot : \mathbb{Q} \rightarrow \mathbb{Q}, [(a, b)] \cdot [(c, d)] = [(ac, bd)]$

It can be proved that this is well defined,

we also have:

- (1)  $a \cdot (b \cdot c) = (a \cdot b) \cdot c$  (Associativity)
- (2)  $a \cdot 1 = a = 1 \cdot a$  (Multiplicative identity)
- (3)  $a \cdot b = b \cdot a$  (Commutativity)
- (4)  $(\forall q \in \mathbb{Q})(\exists! q^{-1} \in \mathbb{Q}) : qq^{-1} = 1$

Proof: (4)

Given  $q = [(a, b)] \neq 0$ ,

$\implies a \neq 0$  Choose  $q^{-1} = [(b, a)]$

Then we have  $qq^{-1} = [(ab, ab)] = 1$

With this all said we define  $[(a, b)] = \frac{a}{b}$

## 1.4 Functions:

Definition: Let  $X, Y \neq \emptyset$ , a function is a relation from  $X$  to  $Y$ ,  $f \subseteq X \times Y$  such that

$$(\forall x \in X)(\exists! y \in Y)((x, y) \in f)$$

We call  $X = \text{Dom}(f), Y = \text{CoDom}(f)$

we write  $f : X \rightarrow Y$  to denote a function from X to Y

also if  $(x, y) \in f$  we write  $f(x) = y$  because the  $y$  is unique,

Definition: If  $f : X \rightarrow Y$  then

$\text{Im}(f) = \{f(x) \mid x \in X\} \subseteq Y$

Example:  $f = \{(x, y) \mid x^2 + y^2 = 1\}$

$f$  is clearly a relation from X to Y but is  $f$  a function?

Solution:

No Since  $x = 0 \implies (0, 1), (0, -1) \in f$

so it violates the uniqueness.

$g = \{(x, y) \mid x \in X, y \in Y, y \geq 0, x^2 + y^2 = 1\}$  Now it is a function.

$h = \{(x, y) \mid x \in [-1, 1], y \in [0, 1], x^2 + y^2 = 1\}$

We see that  $g \neq h$  since the need to have to be identical as sets and that is not true.

Example: Consider  $f : \mathbb{Z}/\sim_n \rightarrow \mathbb{Z}$ .

$f([k]_n) = k$  is not well defined,

$f([0]_n) = 0, f([0]_n = [n]_n) = n$

When defining a function you need your choices to be well defined

Example:  $f : \mathbb{Z}/\sim_6 \rightarrow \mathbb{Z}/\sim_3$

We claim that  $f$  is well defined,

Proof: If  $[a]_6 = [a']_6$  then

$$a \sim_6 a' \implies 6 \mid a - a' \implies 3 \mid a - a'$$

Hence,  $[a]_3 = [a']_3$

Therefore,  $f([a]_6) = f([a']_6)$

Definition: Let  $f : X \rightarrow Y$ ,

Suppose  $A \subseteq X, B \subseteq Y$

(i) The Image of A under  $f$  is

$f(A) := \{f(a) \mid a \in A\}$

(ii) The PreImage of B under  $f$  is

$f^{-1}(B) := \{x \in X \mid f(x) \in B\} \subseteq X$

Notice  $\text{Im}(f) = f(X)$  and  $f^{-1}(B)$  can be empty,

Example:  $f : \mathbb{R} \rightarrow \mathbb{R}, f(x) = x^2$  (i)  $A = [-1, 4], f(A)$ ?

(ii)  $B = \{-1, 2\}, f^{-1}(B)$ ?

(iii)  $f^{-1}((-\infty, 0))$ ? Solution: (i)  $f(A) = \{f(a) \mid a \in A\}$

$= \{a^2 \mid a \in [-1, 4]\} = \{a^2 \mid -1 \leq a \leq 4\}$

so if

$$0 \leq a \leq 4 \iff 0 \leq a^2 \leq 16$$

if

$$-1 \leq a \leq 0 \iff 1 \geq a^2 \geq 0$$

So  $0 \leq a^2 \leq 16$

(ii)  $f^{-1}(B) = \{1, -1, \sqrt{2}, -\sqrt{2}\}$

(iii)  $\emptyset$

Example:

Consider  $\Omega = \{(a_k)_k \mid a_k \in \{0, 1\}\}$

if  $F \subseteq \mathbb{N}$ , is finite, consider  $\sigma_F : \Omega \rightarrow \Omega : \sigma_F((a_k)_k) = (b_k)_k, b_k = \begin{cases} a_k & k \notin F, \\ 1 - a_k & k \in F. \end{cases}$

This just switches the terms of the sequence  $(a_k)_k$  to the opposite if their index is in  $F$

and Recall our equivalence relations on  $\Omega$

$$(a_k)_k \sim (b_k)_k \iff (\exists N \in \mathbb{N})(\forall k \geq N)(a_k = b_k)$$

We claim that  $[\omega] = \{\sigma_F(\omega) \mid F \subseteq \mathbb{N} \text{ finite}\}$

Proof:

Claim 1:  $[\omega] \subseteq \{\sigma_F(\omega) \mid F \subseteq \mathbb{N}\}$

Proof:

$$(x_k)_k \in [\omega] \iff (\exists N \in \mathbb{N}) : (\forall k \geq N)(x_k = \omega_k)$$

Consider the finite set  $\mathcal{F} = \{n \mid n < N\}$

Find  $F \subseteq \mathcal{F} : (x_k) = \sigma_F(\omega)$

hence,  $(x_k) \in \{\sigma_F(\omega) \mid F \subseteq \mathbb{N} \text{ finite}\}$

Claim 2:  $\{\sigma_F(\omega) \mid F \subseteq \mathbb{N} \text{ finite}\} \subseteq [\omega]$

Proof:

$$(x_k)_k \in \{\sigma_F(\omega) \mid F \subseteq \mathbb{N} \text{ finite}\} \iff (\exists F \subseteq \mathbb{N} \text{ finite}) : (\sigma_F(\omega) = (x_k)_k)$$

Since  $F$  is finite we find  $N = \max(F)$

then  $\forall k > N, x_k = \omega_k$

$$\implies (x_k)_k \sim \omega \iff (x_k)_k \in [\omega]$$

Theorem:(Well Definite theorem)

Let  $X, Y \neq \emptyset$  be sets,

and  $\sim$  be an equivalence relations on  $X$

and  $f : X \rightarrow Y$  be any function

If  $x \sim x' \implies f(x) = f(x')$

Then  $\exists! g : X/\sim \rightarrow Y$

We call  $X/\sim$  the quotient space,

Proof: Define  $g([x]_\sim) = f(x)$  We claim that  $g$  is a function(well defined)

Suppose  $(\exists [x] = [x'])$

so  $x \sim x'$  By assumption  $f(x) = f(x')$

Hence  $g([x]) = g([x'])$

So we take  $\pi : X/\sim \rightarrow Y$

and we find that  $f \circ \pi = g$

so  $g : X/\sim \rightarrow Y$  exists.

Uniqueness Suppose we have  $h : X/\sim \rightarrow Y, g([x]) = f(x)$

By definition we have  $h([x]) = g([x])$

Example:  $f : \mathbb{Z} \rightarrow \mathbb{Z} / \sim_6 : f(m) = [2m]_6$ , Suppose that  $m \sim_3 n$ ,

$$3|m-n \iff m-n = 3k \iff 2m-2n = 6k \iff 6|2m-2n \iff [2m]_6 = [2n]_6$$

By Theorem  $\exists! f^* : \mathbb{Z} / \sim_3 \rightarrow \mathbb{Z} / \sim_6$

Example:  $p(x) = \frac{1}{1+x^2}$  give a suitable domain and co-domain, whats the image of  $f$  over its domain?

Solution: We can take  $p : \mathbb{R} \rightarrow \mathbb{R}$ . we claim that  $Im(f) = (0, 1]$ ,

$$1 + x^2 \geq 1 \implies \frac{1}{1+x^2} \leq 1 \text{ and } 0 < \frac{1}{1+x^2} \text{ So } Im(f) \subseteq (0, 1]$$

Now we claim that  $(0, 1] \subseteq Im(f)$

let  $t \in (0, 1]$

$$p(x) = t \iff \frac{1}{1+x^2} = t \iff x^2 + 1 = \frac{1}{t} \iff x^2 = \frac{1}{t} - 1 \iff x = \sqrt{\frac{1}{t} - 1}$$

Proposition: If  $f : X \rightarrow Y$  is a map,  $A \subseteq X, B \subseteq Y$

- (i)  $f(\bigcup_{i \in I} A_i) = \bigcup_{i \in I} f(A_i)$
- (ii)  $f(\bigcap_{i \in I} A_i) \subseteq \bigcap_{i \in I} (f(A_i))$
- (iii)  $f(A^c) \neq f(A)^c$  generally,

Proof:

(i)

$$y \in f\left(\bigcup_{i \in I} A_i\right) \iff (\exists x \in \bigcup_{i \in I} A_i) : (f(x) = y) \iff (\exists i \in I)(\exists x \in A_i) : (f(x) = y)$$

$$\iff (\exists i \in I) : (y \in f(A_i)) \iff y \in \bigcup_{i \in I} f(A_i)$$

(ii)

$$y \in f\left(\bigcap_{i \in I} A_i\right) \implies (\exists x \in \bigcap_{i \in I} A_i) : (\forall i \in I)(y = f(x)) \iff y \in \bigcap_{i \in I} f(A_i)$$

Proposition:

If  $f : X \rightarrow Y$  is a map,  $A \subseteq X, B \subseteq Y$

- (i)  $f^{-1}(\bigcup_{i \in I} A_i) = \bigcup_{i \in I} f^{-1}(A_i)$
- (ii)  $f^{-1}(\bigcap_{i \in I} A_i) = \bigcap_{i \in I} (f^{-1}(A_i))$
- (iii)  $f^{-1}(A^c) = f^{-1}(A)^c$

Proof: (i)

$$\begin{aligned} x \in f^{-1}(\bigcup_{i \in I} A_i) \\ \iff (\exists y \in \bigcup_{i \in I} A_i) : (f(x) = y) \\ \iff (\exists i \in I)(\exists y \in A_i) : (f(x) = y) \\ \iff (\exists i \in I) : (x \in f^{-1}(A_i)) \\ \iff x \in \bigcup_{i \in I} f^{-1}(A_i) \end{aligned}$$

(ii)

$$\begin{aligned} x \in f^{-1}(\bigcap_{i \in I} A_i) \\ \iff (\forall i \in I)(\exists y \in A_i) : (f(x) = y) \\ \iff (\forall i \in I)(x \in f^{-1}(A_i)) \end{aligned}$$

$$\begin{aligned}
&\iff x \in \bigcap_{i \in I} f^{-1}(B_i) \\
&\text{(iii)} \\
&x \in f^{-1}(B^c) \\
&\iff (\exists y \in B^c) : (f(x) = y) \\
&\iff (\exists y \in B) : (f(x) \neq y) \\
&\iff (x \notin f^{-1}(B)) \\
&\iff x \in (f^{-1}(B))^c
\end{aligned}$$

Definition: A function  $f : X \rightarrow Y$  A function  $f : X \rightarrow Y$  is surjective if

$$(\forall y \in Y)(\exists x \in X) : (f(x) = y)$$

equivalently,  $Im(f) = Y$

or  $(\forall y \in Y)(f^{-1}(\{y\}) \neq \emptyset)$

We call  $f^{-1}(\{y\})$  the fiber of  $f$  over  $y$ ,

we have the fibers are disjoint by uniqueness of functions. So we can partition

$$X = \bigsqcup_{y \in Y} f^{-1}(\{y\})$$

Example:  $\pi : \mathbb{Z} \rightarrow \mathbb{Z}/5$

$$\pi^{-1}([1]_5) = 1 + 5\mathbb{Z} \quad \pi^{-1}([2]_5) = 2 + 5\mathbb{Z} \quad \pi^{-1}([3]_5) = 3 + 5\mathbb{Z} \quad \pi^{-1}([4]_5) = 4 + 5\mathbb{Z}$$

$$\pi^{-1}([0]_5) = 5\mathbb{Z} \quad \text{Example: } \lceil x \rceil : \mathbb{R} \rightarrow \mathbb{Z}$$

we have that  $f^{-1}(\{n\}) = (n-1, n]$

$$\text{and } \mathbb{R} = \bigsqcup_{n \in \mathbb{Z}} f^{-1}(\{n\})$$

Proposition: Let  $f : X \rightarrow Y$  be a function,

$$A \subseteq X, B \subseteq Y,$$

$$(i) A \subseteq f^{-1}(f(A))$$

$$(ii) f(f^{-1}(B)) \subseteq B$$

Proof:

(i) Let  $a \in A$

$$\implies f(a) \in f(A) \implies a \in f^{-1}(f(A))$$

(ii)

Let  $y \in f(f^{-1}(B))$

$$\implies y \in f(x), x \in f^{-1}(B) \implies y \in B$$

The Algebra of Functions:

Fix  $S \neq \emptyset$ ,

(i)  $id_S : S \rightarrow S, id_S(x) = x$

$$(ii) \text{ Let } A \in S, \mathbb{1}_A := \begin{cases} 1 & x \in A \\ 0 & x \notin A \end{cases}$$

if  $A = \{a\}$

we says that  $\mathbb{1}_{\{a\}} = \delta_a$

Example: Consider  $\mathbb{1}_A, \mathbb{1}_B : S \rightarrow \mathbb{R}$

$$\mathbb{1}_A = \mathbb{1}_B \iff A = B$$

Proof: We see that  $\mathbb{1}_A = \mathbb{1}_B \iff A = \mathbb{1}_B, (\forall x \in \Omega)$

So if  $x \in A \iff \mathbb{1}_A = 1$

$$\iff 1 = \mathbb{1} \iff x \in B$$

Hence  $A = B$

Definition: Fix  $S \neq \emptyset$ , Let  $\mathcal{F}(S, \mathbb{R}) = \{f \mid f : S \rightarrow \mathbb{R}\}$   
for  $f, g \in \mathcal{F}(S, \mathbb{R}), t \in \mathbb{R}$ , Define

$$(i)(f \pm g)(x) = f(x) \pm g(x)$$

$$(ii)(tf)(x) = tf(x)$$

$$(iii)(fg)(x) = f(x)g(x)$$

If  $g(x) \neq 0, \forall x \in S$

$$(iv)\frac{1}{g}(x) = \frac{1}{g(x)}$$

We says that  $\mathbb{1}_\emptyset = 0$

and  $\mathbb{1}_S = 1$

Example:  $\mathbb{1}_A \cdot \mathbb{1}_B = \mathbb{1}_{A \cap B}$

Proof: Let  $x \in S$

if  $x \in A \cap B$

then  $\mathbb{1}_{A \cap B}(x) = 1$

and  $\mathbb{1}_A \cdot \mathbb{1}_B = 1$

Without loss of generality,  $x \in A, x \notin B$

then  $\mathbb{1}_{A \cap B}(x) = 0$

and  $\mathbb{1}_A \cdot \mathbb{1}_B = 0$

We notice also  $\mathbb{1}_{A \cup B} = \mathbb{1}_A + \mathbb{1}_B - \mathbb{1}_{A \cap B}$

Definition: Let  $f \in \mathcal{F}(S, \mathbb{R})$

if  $Im(f)$  is finite then we call f simple.

Example: if  $im(f) = \{a_1, a_2, \dots, a_n\}$

we can express  $f = \sum_{k=1}^n a_k \mathbb{1}_{f^{-1}(\{a_k\})}$

Composition of Functions:

Definition: Let  $f : X \rightarrow Y, g : Y \rightarrow Z$

We define  $g \circ f : X \rightarrow Z, g(f(x))$

Note that  $im(f) \subseteq Dom(g)$

## 1.5 A Glimpse of Probability

Throughout, Let  $\Omega$  be a finite set, we can refer to  $\Omega$  as the sample space.

Example: Consider  $\Omega := \{(x, y) \mid 1 \leq x \leq 6, 1 \leq y \leq 6\} = \{(1, 1), (1, 2), \dots, (1, 6), (2, 1), \dots, (6, 6)\}$

Notice that this can be interpreted as the set of all possible ways to roll two distinguishable dice.  $|\Omega| = 36$  and the "Probability" of getting an outcome is

$\frac{1}{36}$  for any combinations. Definition:

If  $P : \Omega \rightarrow [0, 1] : \sum_{x \in \Omega} P(x) = 1$  then we call P a probability function on  $\Omega$

In our above example we see that  $P(i, j) = \frac{1}{36}$  we call this a uniform probability.

Given a probability function we wish to talk about a probability measure. i.e. we wish to find the probability of a subset of events rather than a single one.

In the dice example consider  $E = \{(i, j) \in \Omega \mid i + j = 5\}$  what is the likelihood of  $i + j = 5$ ? In this example we can just list them out and see we have 4 elements

in  $E$  and hence  $\frac{4}{36}$

Definition:

If  $\mu : \mathcal{P}(\Omega) \rightarrow [0, 1]$  meaning  $(\forall E \subseteq \Omega)(E \mapsto \mu(E) \in [0, 1])$  with the following properties:

(i)  $\mu(\emptyset) = 0$

(ii)  $\mu(\Omega) = 1$

(iii) if  $\{E_i\}_{i \in I}$  is a pairwise disjoint family of subsets of  $\Omega$

then  $\mu(\bigsqcup_{i \in I} E_i) = \sum_{i \in I} \mu(E_i)$

Then we call  $\mu$  a probability measure on  $\Omega$

So given a probability functions  $P : \Omega \rightarrow [0, 1]$  we get  $\mu_P : \mathcal{P}(\Omega) \rightarrow [0, 1]$

a probability measure with  $\mu_P(E) = \sum_{w \in E} P(w)$

In the above example where  $E = \{(i, j) \in \Omega \mid i + j = 5\}$ ,  $\mu_P(E) = \frac{1}{9}$

Proposition:  $\mu(E^c) = 1 - \mu(E)$

Proof:  $E^c \cap E = \emptyset, E^c \cup E = \Omega \implies E^c \sqcup E = \Omega$

Hence,

$$1 = \mu(\Omega) = \mu(E^c \sqcup E) = \mu(E^c) + \mu(E) \iff \mu(E^c) = 1 - \mu(E)$$